store/client_proofs/connect.v
@@ -45,7 +45,8 @@ iIntros "#chan_c #ctx #ctx'".
 iPoseProof (store_ctx_conn_ctx with "ctx'") as "?".
 iIntros "#p_ekI #p_ekR".
 iIntros "!> %Φ client post".
-iDestruct "client" as "(%n & %failed & db & dis)".
+iDestruct "client"
+  as "(%n & %failed & %db & dis & version & #db_at & state)".
 wp_lam. wp_pures.
 iApply (Conn.wp_connect with "[//] [//] [//] [//] [//] [$]") => //.
 iIntros "!> %cs (conn & token)".
